our_cook/completeness.v
@@ -1,0 +1,6 @@
+Theorem complete: forall s P u r, 
+  (encode s u r []) -( a_tau )> P -> 
+  exists P' t,
+    P =()> P' /\ (P' ~~ encode t u r []) /\ (s --> t \/ s = t).
+Proof.
+Admitted.
